tools/Vale/test/Vale.fst
@@ -7,7 +7,7 @@ open FStar.Map
 (***** Vale Interface *****)
 
 (*
- * Aseems says, "what are the access qualifiers on Semantics and this interface?"
+ * Aseem says, "what are the access qualifiers on Semantics and this interface?"
  *)
 
 (* Type aliases *)
@@ -25,10 +25,10 @@ type va_register = reg
 
 (* Constructors *)
 let va_op_operand_reg (r:reg) :va_operand = OReg r
-let va_const_operand (n:nat64) = OConst n
-let va_const_shift_amt (n:nat64) :va_shift_amt = OConst n
+let va_const_operand (n:nat{normalize (n < pow2 64)}) = OConst (FStar.UInt64.uint_to_t n)
+let va_const_shift_amt (n:nat{normalize (n < pow2 64)}) :va_shift_amt = OConst (FStar.UInt64.uint_to_t n)
 let va_op_cmp_reg (r:reg) :va_cmp = OReg r
-let va_const_cmp (n:nat64) :va_cmp = OConst n
+let va_const_cmp (n:nat{normalize (n < pow2 64)}) :va_cmp = OConst (FStar.UInt64.uint_to_t n)
 let va_coerce_register_to_operand (r:va_register) :va_operand = OReg r
 let va_op_register (r:reg) :va_register = r
 let va_op_dst_operand_reg (r:reg{ not (Rsp? r) }) : va_dst_operand = OReg r
@@ -39,8 +39,8 @@ let va_coerce_dst_operand_to_operand (o:va_dst_operand) : va_operand = o
 let va_is_src_operand_uint64 (o:operand) (s:va_state) = valid_operand o s
 let va_is_dst_operand_uint64 (o:operand) (s:va_state) = valid_dst o
 let va_is_dst_dst_operand_uint64 (o:va_dst_operand) (s:va_state) = valid_operand o s
-let va_is_src_register_int (r:reg) (s:va_state) :bool = true
-let va_is_dst_register (r:reg) (s:va_state) :bool = true
+let va_is_src_register_int (r:reg) (s:va_state) = true
+let va_is_dst_register (r:reg) (s:va_state) = true
 let va_is_src_shift_amt_uint64 (o:operand) (s:va_state) = valid_shift_operand o s
 
 (* Getters *)
@@ -63,29 +63,27 @@ let va_update_dst_operand (o:dst_op) (sM:va_state) (sK:va_state) :va_state =
   va_update_operand o sM sK   
 let va_update_register (r:reg) (sM:va_state) (sK:va_state) :va_state = va_update_reg r sM sK
 
-open FStar.UInt64
-
 (* Evaluation *)
-let va_eval_operand_uint64 (s:va_state) (o:va_operand) :int = v (eval_operand o s)
-let va_eval_dst_operand_uint64 (s:va_state) (o:va_dst_operand) :int = v (eval_operand o s)
-let va_eval_shift_amt_uint64 (s:va_state) (o:va_shift_amt) : int = v (eval_operand o s)
-let va_eval_cmp_uint64 (s:va_state) (r:va_cmp) :int = v (eval_operand r s)
-let va_eval_register_uint64 (s:va_state) (r:va_register) :int = v (eval_reg r s)
-
+let va_eval_operand_uint64     (s:va_state) (o:va_operand)     :int = FStar.UInt64.v (eval_operand o s)
+let va_eval_dst_operand_uint64 (s:va_state) (o:va_dst_operand) :int = FStar.UInt64.v (eval_operand o s)
+let va_eval_shift_amt_uint64   (s:va_state) (o:va_shift_amt)   :int = FStar.UInt64.v (eval_operand o s)
+let va_eval_cmp_uint64         (s:va_state) (r:va_cmp)         :int = FStar.UInt64.v (eval_operand r s)
+let va_eval_register_uint64    (s:va_state) (r:va_register)    :int = FStar.UInt64.v (eval_reg r s)
 
 (* Dealing with code *)
-let va_CNil () :va_codes = []
-let va_CCons (hd:va_code) (tl:va_codes) :va_codes = hd::tl
-let va_Block (block:va_codes) :va_code = Block block
-let va_IfElse (ifCond:ocmp) (ifTrue:va_code) (ifFalse:va_code) :va_code = IfElse ifCond ifTrue ifFalse
-let va_While (whileCond:ocmp) (whileBody:va_code) (inv:operand) :va_code = While whileCond whileBody inv
-let va_cmp_le (a:va_operand) (b:va_operand) :ocmp = OLe a b
-let va_get_block (c:va_code{Block? c}) :va_codes = Block?.block c
-let va_get_ifCond (c:code{IfElse? c}) :ocmp = IfElse?.ifCond c
-let va_get_ifTrue (c:code{IfElse? c}) :code = IfElse?.ifTrue c
-let va_get_ifFalse (c:code{IfElse? c}) :code = IfElse?.ifFalse c
-let va_get_whileCond (c:code{While? c}) :ocmp = While?.whileCond c
-let va_get_whileBody (c:code{While? c}) :code = While?.whileBody c
+let va_CNil ()                                                  :va_codes = []
+let va_CCons (hd:va_code) (tl:va_codes)                         :va_codes = hd::tl
+let va_Block (block:va_codes)                                   :va_code  = Block block
+let va_IfElse (ifCond:ocmp) (ifTrue:va_code) (ifFalse:va_code)  :va_code  = IfElse ifCond ifTrue ifFalse
+let va_While (whileCond:ocmp) (whileBody:va_code) (inv:operand) :va_code  = While whileCond whileBody inv
+let va_cmp_le (a:va_operand) (b:va_operand)                     :ocmp     = OLe a b
+
+let va_get_block (c:va_code{Block? c})  :va_codes = Block?.block c
+let va_get_ifCond (c:code{IfElse? c})   :ocmp     = IfElse?.ifCond c
+let va_get_ifTrue (c:code{IfElse? c})   :code     = IfElse?.ifTrue c
+let va_get_ifFalse (c:code{IfElse? c})  :code     = IfElse?.ifFalse c
+let va_get_whileCond (c:code{While? c}) :ocmp     = While?.whileCond c
+let va_get_whileBody (c:code{While? c}) :code     = While?.whileBody c
 
 
 let va_state_eq (s_0:va_state) (s_1:va_state) :Type0 = 
@@ -107,8 +105,7 @@ let va_ensure (b_0:va_codes) (b_1:va_codes) (s_0:va_state) (s_1:va_state) (sN:va
 
 (* the lemmas have out variables, so writing them as pure functions *)
 
-(* abstract? *)
-
+abstract
 let va_lemma_block (b_0:va_codes) (s_0:state) (sN:state)
   :Pure (state * va_code * va_codes)
         (requires (Cons? b_0 /\ Some(sN) == eval_code (Block b_0) s_0))
@@ -118,11 +115,13 @@ let va_lemma_block (b_0:va_codes) (s_0:state) (sN:state)
   = let c_1::b_1 = b_0 in
     Some?.v (eval_code c_1 s_0), c_1, b_1
 
+abstract
 let va_lemma_empty (s_0:va_state) (sN:va_state)
   :Pure va_state (requires (Some(sN) == eval_code (Block (va_CNil ())) s_0))
                  (ensures  (fun sM -> sM == s_0 /\ sM == sN))
   = s_0
 
+abstract
 let va_lemma_ifElse (ifb:ocmp) (ct:code) (cf:code) (s_0:va_state) (sN:va_state)
   :Pure (bool * va_state)
         (requires (Some(sN) == eval_code (IfElse ifb ct cf) s_0))
@@ -136,12 +135,14 @@ let va_whileInv (b:ocmp) (c:code{While? c}) (inv:operand) (s_0:va_state) (sN:va_
   va_eval_operand_uint64 s_0 inv >= 0 /\
   Some(sN) == eval_while c s_0
 
+abstract
 let va_lemma_while (b:ocmp) (c:code) (inv:operand) (s_0:va_state) (sN:va_state)
   :Pure va_state
         (requires (Some(sN) == eval_code (While b c inv) s_0))
 	(ensures  (fun s_1 -> Some(sN) == eval_while (While b c inv) s_0 /\ s_1 == s_0))
   = s_0
 
+abstract
 let va_lemma_whileTrue (b:ocmp) (c:code) (inv:operand) (s_0:va_state) (sN:va_state)
   :Pure (va_state * va_state)
         (requires (va_eval_operand_uint64 s_0 inv > 0 /\
@@ -152,6 +153,7 @@ let va_lemma_whileTrue (b:ocmp) (c:code) (inv:operand) (s_0:va_state) (sN:va_sta
 				  (if s_1.ok then Some(sN) == eval_while (While b c inv) s_1 else s_1 == sN)))
   = s_0, Some?.v (eval_code c s_0)
 
+abstract
 let va_lemma_whileFalse (b:ocmp) (c:code) (inv:operand) (s_0:va_state) (sN:va_state)
   :Pure va_state (requires (eval_operand inv s_0 == 0uL /\
                             Some(sN) == eval_while (While b c inv) s_0))
